Clean/Circuit/Lawful.lean
@@ -294,6 +294,6 @@ theorem bind_completeness {f : Circuit F α} {g : α → Circuit F β} (f_lawful
   simp only [completeness_iff_generic, bind_generic]
 end Circuit.constraints_hold
 
-attribute [lawful_norm] LawfulCircuit.final_offset LawfulCircuit.operations LawfulCircuit.output
+attribute [lawful_norm] LawfulCircuit.final_offset LawfulCircuit.operations LawfulCircuit.output ConstantLawfulCircuit.local_length
 attribute [lawful_norm] ConstantLawfulCircuits.output ConstantLawfulCircuits.local_length ConstantLawfulCircuits.operations
   ConstantLawfulCircuits.from_constant_length id_eq
